Align Logos cardinality proofs with SQL integrity semantics
Framework: Consume the FormalSQL-owned schema-constraint interface and remove the duplicate Logos constraint module.

Proof: Bridge typed non-NULL INT32 SQL equality to structural cardinality bounds, with regression coverage and agent-facing lemma guidance.

tests/rocq/regressions/SchemaRegression.v
@@ -1,8 +1,9 @@
-From Stdlib Require Import Lia List String ZArith.
+From Stdlib Require Import Lia List SetoidList String ZArith.
 From SQLFS Require Import
   SqlSyntax GenericInstance Values FTuples FiniteBag FiniteCollection
-  FiniteSet OrderedSet ValueInteger.
-From Logos.FormalSQL Require Import SchemaConstraints SchemaCardinality.
+  FiniteSet OrderedSet ValueInteger Bool3 SqlErrorSemantics SchemaConstraints.
+From Logos.FormalSQL Require Import
+  TNullSyntax SchemaCardinality.
 
 Import ListNotations.
 Import Tuple.
@@ -22,6 +23,31 @@ Definition regression_null_key_row (payload : Z) : tuple TNull :=
     [regression_key; regression_payload]
     [Value_Z None; Value_Z (Some payload)].
 
+Definition regression_optional_row
+    (key payload : option Z) : tuple TNull :=
+  mk_tuple_lists
+    [regression_key; regression_payload]
+    [Value_Z key; Value_Z payload].
+
+Lemma regression_NoDupA_two :
+  forall (A : Type) (relation : A -> A -> Prop) left right,
+    ~ relation left right ->
+    NoDupA relation [left; right].
+Proof.
+intros A relation left right Hdistinct.
+constructor.
+- intro Hin.
+  apply InA_alt in Hin as [value [Hrelated Hvalue]].
+  cbn in Hvalue.
+  destruct Hvalue as [-> | []].
+  now apply Hdistinct.
+- constructor.
+  + intro Hin.
+    apply InA_alt in Hin as [value [_ Hvalue]].
+    now inversion Hvalue.
+  + constructor.
+Qed.
+
 Example duplicate_primary_key_is_rejected :
   ~ primary_key_conforms
       [regression_key]
@@ -29,7 +55,10 @@ Example duplicate_primary_key_is_rejected :
 Proof.
 intros [_ [_ Hnodup]].
 inversion Hnodup as [| projected remaining Hnotin _].
-apply Hnotin; left; reflexivity.
+apply Hnotin.
+apply InA_cons_hd.
+vm_compute.
+split; [reflexivity|exact I].
 Qed.
 
 Example null_primary_key_is_rejected :
@@ -45,6 +74,502 @@ specialize
     regression_key
     (or_introl eq_refl)).
 vm_compute in Hnot_null; discriminate.
+Qed.
+
+Example duplicate_ordinary_unique_key_is_rejected :
+  ~ unique_key_conforms
+      [regression_key]
+      [regression_row 1 10; regression_row 1 20].
+Proof.
+intros [_ Hnodup].
+inversion Hnodup as [| projected remaining Hnotin _].
+apply Hnotin.
+apply InA_cons_hd.
+vm_compute.
+split; [reflexivity|exact I].
+Qed.
+
+Example ordinary_unique_nulls_are_distinct :
+  unique_key_conforms
+    [regression_key]
+    [regression_null_key_row 10; regression_null_key_row 20].
+Proof.
+split; [discriminate|].
+apply regression_NoDupA_two.
+vm_compute.
+intros [Hequal _]; discriminate.
+Qed.
+
+Example composite_unique_null_component_is_distinct :
+  unique_key_conforms
+    [regression_key; regression_payload]
+    [regression_optional_row (Some 1) None;
+     regression_optional_row (Some 1) None].
+Proof.
+split; [discriminate|].
+apply regression_NoDupA_two.
+vm_compute.
+intros [_ [Hequal _]]; discriminate.
+Qed.
+
+Definition regression_foreign_key : foreign_key_constraint :=
+  ForeignKeyConstraint
+    [regression_key]
+    (Rel "parent")
+    [regression_key].
+
+Definition regression_composite_foreign_key : foreign_key_constraint :=
+  ForeignKeyConstraint
+    [regression_key; regression_payload]
+    (Rel "composite_parent")
+    [regression_key; regression_payload].
+
+Example match_simple_matching_row_satisfies_foreign_key :
+  foreign_key_row_conforms_against
+    regression_foreign_key
+    (regression_row 1 20)
+    [regression_row 1 10].
+Proof.
+eapply foreign_key_match_simple_referenced_row with
+  (referenced_row := regression_row 1 10).
+- now left.
+- vm_compute.
+  repeat split; try reflexivity; exact I.
+Qed.
+
+Example match_simple_null_component_satisfies_foreign_key :
+  foreign_key_row_conforms_against
+    regression_foreign_key
+    (regression_null_key_row 20)
+    nil.
+Proof.
+eapply foreign_key_match_simple_null_component with
+  (attribute := regression_key).
+- now left.
+- reflexivity.
+Qed.
+
+Example match_simple_composite_any_null_component_satisfies_foreign_key :
+  foreign_key_row_conforms_against
+    regression_composite_foreign_key
+    (regression_optional_row (Some 1) None)
+    nil.
+Proof.
+eapply foreign_key_match_simple_null_component with
+  (attribute := regression_payload).
+- now right; left.
+- reflexivity.
+Qed.
+
+Example unmatched_nonnull_row_violates_foreign_key :
+  ~ foreign_key_row_conforms_against
+      regression_foreign_key
+      (regression_row 2 20)
+      [regression_row 1 10].
+Proof.
+intros [[attribute [Hattribute Hnull]] |
+  [referenced_row [Hrow Hequal]]].
+- cbn in Hattribute.
+  destruct Hattribute as [<- | []].
+  vm_compute in Hnull; discriminate.
+- cbn in Hrow.
+  destruct Hrow as [<- | []].
+  vm_compute in Hequal.
+  intuition discriminate.
+Qed.
+
+Definition regression_parent_constraint : table_constraint :=
+  TableConstraint
+    (Rel "parent") [regression_key] (Some [regression_key])
+    nil nil nil nil.
+
+Definition regression_child_constraint : table_constraint :=
+  TableConstraint
+    (Rel "child") nil None nil [regression_foreign_key] nil nil.
+
+Example referenced_primary_key_is_well_formed :
+  foreign_key_reference_well_formed
+    [regression_parent_constraint; regression_child_constraint]
+    regression_foreign_key.
+Proof.
+unfold foreign_key_reference_well_formed.
+cbn [regression_foreign_key].
+split; [discriminate|].
+split; [reflexivity|].
+split.
+- constructor; [reflexivity|constructor].
+- exists regression_parent_constraint.
+  split; [now left|].
+  split; [reflexivity|now left].
+Qed.
+
+Definition regression_unique_parent_constraint : table_constraint :=
+  TableConstraint
+    (Rel "parent") nil None [[regression_key]] nil nil nil.
+
+Example referenced_ordinary_unique_key_is_well_formed :
+  foreign_key_reference_well_formed
+    [regression_unique_parent_constraint; regression_child_constraint]
+    regression_foreign_key.
+Proof.
+unfold foreign_key_reference_well_formed.
+cbn [regression_foreign_key].
+split; [discriminate|].
+split; [reflexivity|].
+split.
+- constructor; [reflexivity|constructor].
+- exists regression_unique_parent_constraint.
+  split; [now left|].
+  split; [reflexivity|now right; left].
+Qed.
+
+Definition regression_nonunique_parent_constraint : table_constraint :=
+  TableConstraint (Rel "parent") nil None nil nil nil nil.
+
+Example foreign_key_to_nonunique_columns_is_malformed :
+  ~ foreign_key_reference_well_formed
+      [regression_nonunique_parent_constraint]
+      regression_foreign_key.
+Proof.
+intros [_ [_ [_
+  [referenced_constraint [Hconstraint [_ Hunique]]]]]].
+cbn in Hconstraint.
+destruct Hconstraint as [<- | []].
+cbn [table_declares_unique_key
+  regression_nonunique_parent_constraint] in Hunique.
+destruct Hunique as [Hprimary | Hordinary].
+- discriminate.
+- contradiction.
+Qed.
+
+Definition regression_int32_one : int32.
+Proof.
+refine (Int32 1 _); unfold int32_min, int32_max; lia.
+Defined.
+
+Definition regression_int64_one : int64.
+Proof.
+refine (Int64 1 _); unfold int64_min, int64_max; lia.
+Defined.
+
+Definition regression_child_int32 : attribute TNull :=
+  Attr_int32 "child_id".
+
+Definition regression_parent_int64 : attribute TNull :=
+  Attr_int64 "parent_id".
+
+Definition regression_int32_row : tuple TNull :=
+  mk_tuple_lists
+    [regression_child_int32]
+    [NullValues.Value_int32 (Some regression_int32_one)].
+
+Definition regression_int64_row : tuple TNull :=
+  mk_tuple_lists
+    [regression_parent_int64]
+    [NullValues.Value_int64 (Some regression_int64_one)].
+
+Definition regression_cross_integral_foreign_key : foreign_key_constraint :=
+  ForeignKeyConstraint
+    [regression_child_int32]
+    (Rel "big_parent")
+    [regression_parent_int64].
+
+Example cross_integral_foreign_key_components_are_compatible :
+  Forall2 foreign_key_attribute_compatible
+    [regression_child_int32] [regression_parent_int64].
+Proof.
+constructor.
+- apply foreign_key_attribute_compatible_int32_int64.
+- constructor.
+Qed.
+
+Example heterogeneous_string_foreign_key_components_fail_closed :
+  ~ foreign_key_attribute_compatible
+      (Attr_string "child" StringText)
+      (Attr_string "parent" (StringChar 4)).
+Proof.
+cbn; discriminate.
+Qed.
+
+Example cross_integral_equal_payload_satisfies_foreign_key :
+  foreign_key_row_conforms_against
+    regression_cross_integral_foreign_key
+    regression_int32_row
+    [regression_int64_row].
+Proof.
+eapply foreign_key_match_simple_referenced_row with
+  (referenced_row := regression_int64_row).
+- now left.
+- cbn [regression_cross_integral_foreign_key
+    foreign_key_key_equal_true regression_int32_row
+    regression_int64_row].
+  split.
+  + apply foreign_key_value_equal_true_int32_int64.
+    reflexivity.
+  + exact I.
+Qed.
+
+Definition regression_positive_payload_formula : Formula :=
+  Pred PredicateGt
+    [AExpr (Dot regression_payload);
+     AExpr (Constant (Value_Z (Some 0)))].
+
+Definition regression_positive_payload_check : check_constraint :=
+  CheckConstraint regression_positive_payload_formula.
+
+Example check_true_satisfies_constraint :
+  check_row_conforms
+    init_db regression_positive_payload_check (regression_row 1 10).
+Proof.
+vm_compute.
+split; [reflexivity|discriminate].
+Qed.
+
+Example check_unknown_satisfies_constraint :
+  check_row_conforms
+    init_db regression_positive_payload_check
+    (regression_optional_row (Some 1) None).
+Proof.
+vm_compute.
+split; [reflexivity|discriminate].
+Qed.
+
+Example check_false_violates_constraint :
+  ~ check_row_conforms
+      init_db regression_positive_payload_check (regression_row 1 (-10)).
+Proof.
+vm_compute.
+intros [_ Hnot_false]; now apply Hnot_false.
+Qed.
+
+Definition regression_int32_zero : int32.
+Proof.
+refine (Int32 0 _); unfold int32_min, int32_max; lia.
+Defined.
+
+Definition regression_division_by_zero_formula : Formula :=
+  Pred PredicateEq
+    [AScalarCall (ScalarDivide ScalarInt32)
+       [AExpr
+          (Constant
+            (NullValues.Value_int32 (Some regression_int32_one)));
+        AExpr
+          (Constant
+            (NullValues.Value_int32 (Some regression_int32_zero)))];
+     AExpr
+       (Constant (NullValues.Value_int32 (Some regression_int32_one)))].
+
+Definition regression_error_check : check_constraint :=
+  CheckConstraint regression_division_by_zero_formula.
+
+Example check_evaluation_error_violates_constraint :
+  ~ check_row_conforms init_db regression_error_check (regression_row 1 10).
+Proof.
+intros [Herror _].
+vm_compute in Herror; discriminate.
+Qed.
+
+Definition regression_key_index_term : constraint_term :=
+  Dot regression_key.
+
+Definition regression_partial_positive_index : unique_index_constraint :=
+  UniqueIndexConstraint
+    [regression_key_index_term]
+    (Some regression_positive_payload_formula).
+
+Example duplicate_participating_partial_index_key_is_rejected :
+  ~ unique_index_conforms
+      init_db
+      [regression_row 1 10; regression_row 1 20]
+      regression_partial_positive_index.
+Proof.
+intros [_ [_ [_ Hnodup]]].
+assert (Hfirst_participates :
+  unique_index_row_participates init_db regression_partial_positive_index
+    (regression_row 1 10) = true) by reflexivity.
+assert (Hsecond_participates :
+  unique_index_row_participates init_db regression_partial_positive_index
+    (regression_row 1 20) = true) by reflexivity.
+cbn [filter] in Hnodup.
+rewrite Hfirst_participates, Hsecond_participates in Hnodup.
+cbn [map] in Hnodup.
+inversion Hnodup as [| projected remaining Hnotin _].
+apply Hnotin.
+apply InA_cons_hd.
+change
+  (sql_value_equal_true (Value_Z (Some 1)) (Value_Z (Some 1)) /\ True).
+split; [reflexivity|exact I].
+Qed.
+
+Example false_predicate_rows_do_not_participate_in_partial_index :
+  unique_index_conforms
+    init_db
+    [regression_row 1 (-10); regression_row 1 (-20)]
+    regression_partial_positive_index.
+Proof.
+unfold unique_index_conforms.
+split; [discriminate|].
+split.
+- intros row Hrow.
+  cbn in Hrow.
+  destruct Hrow as [<- | [<- | []]]; reflexivity.
+- split.
+  + intros row Hrow Hparticipates.
+    cbn in Hrow.
+    destruct Hrow as [<- | [<- | []]];
+      change (false = true) in Hparticipates; discriminate.
+  + assert (Hfirst :
+      unique_index_row_participates init_db regression_partial_positive_index
+        (regression_row 1 (-10)) = false) by reflexivity.
+    assert (Hsecond :
+      unique_index_row_participates init_db regression_partial_positive_index
+        (regression_row 1 (-20)) = false) by reflexivity.
+    cbn [filter].
+    now rewrite Hfirst, Hsecond; constructor.
+Qed.
+
+Example unknown_predicate_rows_do_not_participate_in_partial_index :
+  unique_index_conforms
+    init_db
+    [regression_optional_row (Some 1) None;
+     regression_optional_row (Some 1) None]
+    regression_partial_positive_index.
+Proof.
+unfold unique_index_conforms.
+split; [discriminate|].
+split.
+- intros row Hrow.
+  cbn in Hrow.
+  destruct Hrow as [<- | [<- | []]]; reflexivity.
+- split.
+  + intros row Hrow Hparticipates.
+    cbn in Hrow.
+    destruct Hrow as [<- | [<- | []]];
+      change (false = true) in Hparticipates; discriminate.
+  + assert (Hfirst :
+      unique_index_row_participates init_db regression_partial_positive_index
+        (regression_optional_row (Some 1) None) = false) by reflexivity.
+    cbn [filter].
+    now rewrite Hfirst; constructor.
+Qed.
+
+Definition regression_error_index_term : constraint_term :=
+  ScalarCall (ScalarDivide ScalarInt32)
+    [Constant (NullValues.Value_int32 (Some regression_int32_one));
+     Constant (NullValues.Value_int32 (Some regression_int32_zero))].
+
+Definition regression_error_expression_index : unique_index_constraint :=
+  UniqueIndexConstraint [regression_error_index_term] None.
+
+Example participating_index_expression_error_is_rejected :
+  ~ unique_index_conforms
+      init_db [regression_row 1 10] regression_error_expression_index.
+Proof.
+intros [_ [_ [Hterms _]]].
+specialize Hterms with
+  (row := regression_row 1 10) (1 := or_introl eq_refl) (2 := eq_refl).
+unfold unique_index_row_terms_succeed in Hterms.
+inversion Hterms as [|term terms Herror _].
+vm_compute in Herror; discriminate.
+Qed.
+
+Definition regression_nonparticipating_error_expression_index
+    : unique_index_constraint :=
+  UniqueIndexConstraint
+    [regression_error_index_term]
+    (Some regression_positive_payload_formula).
+
+Example nonparticipating_index_expression_error_is_irrelevant :
+  unique_index_conforms
+    init_db
+    [regression_row 1 (-10)]
+    regression_nonparticipating_error_expression_index.
+Proof.
+unfold unique_index_conforms.
+split; [discriminate|].
+split.
+- intros row Hrow.
+  cbn in Hrow.
+  destruct Hrow as [<- | []]; reflexivity.
+- split.
+  + intros row Hrow Hparticipates.
+    cbn in Hrow.
+    destruct Hrow as [<- | []].
+    change (false = true) in Hparticipates; discriminate.
+  + assert (Hrow :
+      unique_index_row_participates init_db
+        regression_nonparticipating_error_expression_index
+        (regression_row 1 (-10)) = false) by reflexivity.
+    cbn [filter].
+    now rewrite Hrow; constructor.
+Qed.
+
+Definition regression_error_predicate_index : unique_index_constraint :=
+  UniqueIndexConstraint
+    [regression_key_index_term]
+    (Some regression_division_by_zero_formula).
+
+Example partial_index_predicate_error_is_rejected :
+  ~ unique_index_conforms
+      init_db [regression_row 1 10] regression_error_predicate_index.
+Proof.
+intros [_ [Hpredicate_error _]].
+specialize Hpredicate_error with
+  (row := regression_row 1 10) (1 := or_introl eq_refl).
+vm_compute in Hpredicate_error; discriminate.
+Qed.
+
+Definition regression_is_null_index : unique_index_constraint :=
+  UniqueIndexConstraint
+    [regression_key_index_term]
+    (Some (Pred PredicateIsNull [AExpr (Dot regression_key)])).
+
+Example is_null_partial_index_participates_only_on_true :
+  unique_index_row_participates
+    init_db regression_is_null_index (regression_null_key_row 10) = true /\
+  unique_index_row_participates
+    init_db regression_is_null_index (regression_row 1 10) = false.
+Proof.
+split; reflexivity.
+Qed.
+
+Definition regression_name : attribute TNull :=
+  Attr_string "name" StringText.
+
+Definition regression_name_row (name : string) : tuple TNull :=
+  mk_tuple_lists
+    [regression_name]
+    [NullValues.Value_string (StringValue StringText (Some name))].
+
+Definition regression_lower_name_term : constraint_term :=
+  ScalarCall (ScalarStringCase ScalarLower) [Dot regression_name].
+
+Definition regression_lower_name_index : unique_index_constraint :=
+  UniqueIndexConstraint [regression_lower_name_term] None.
+
+Example lower_expression_index_evaluates_the_indexed_expression :
+  unique_index_key
+    [regression_lower_name_term] (regression_name_row "A") =
+  [NullValues.Value_string (StringValue StringText (Some "a"))].
+Proof.
+reflexivity.
+Qed.
+
+Definition regression_empty_index : unique_index_constraint :=
+  UniqueIndexConstraint nil None.
+
+Definition regression_malformed_table_constraint : table_constraint :=
+  TableConstraint
+    (Rel "malformed") nil None [nil] nil nil [regression_empty_index].
+
+Example empty_unique_and_index_keys_are_malformed :
+  ~ table_constraint_declarations_well_formed
+      [regression_malformed_table_constraint]
+      regression_malformed_table_constraint.
+Proof.
+intros [_ [Hunique _]].
+inversion Hunique as [|key keys Hnonempty _].
+now apply Hnonempty.
 Qed.
 
 (** This interface check avoids rebuilding a large concrete finite-domain
